theories/Dot/semtyp_lemmas/tproj_lr.v
@@ -360,11 +360,7 @@ Section type_proj.
 
     iIntros "!> %ρ %v #HT"; rewrite oProjN_eq.
     iAssert (oTMemL A T T anil ρ auxV.[ρ])%I as "{HwT} #Hw". {
-      rewrite -(path_wp_pv_eq auxV.[ρ]).
-      iSpecialize ("HwT" $! ρ with "[//]").
-      iApply (path_wp_proper with "HwT").
-      move=>?/=. f_equiv=> d.
-      by rewrite !oDTMem_unfold.
+      rewrite -(path_wp_pv_eq auxV.[ρ]). by iApply "HwT".
     }
 
     iExists auxV.[ρ]; iFrame "Hw".
